secure_api/merkle_tree/LowStar.Buffer.Generic.fst
@@ -1,0 +1,80 @@
+module LowStar.Buffer.Generic
+
+include LowStar.Monotonic.Buffer.Generic
+
+module Seq = FStar.Seq
+module HST = FStar.HyperStack.ST
+
+(*
+ * Wrapper over LowStar.Monotonic.Buffer, with trivial preorders
+ *   -- functions that take explicit preorder as arguments (e.g. sub etc.)
+ *   -- these include allocation functions also
+ *)
+private let trivial_preorder (a:Type0) :srel a = fun _ _ -> True
+
+type buffer (a:Type0) (st:eqtype) = mbuffer a st (trivial_preorder a) (trivial_preorder a)
+
+unfold let null (#a:Type0) (#st:eqtype) :buffer a st = mnull #a #st #(trivial_preorder a) #(trivial_preorder a)
+
+unfold let gsub (#a:Type0) (#st:eqtype) = mgsub #a #st #(trivial_preorder a) #(trivial_preorder a) (trivial_preorder a)
+
+unfold let gsub_inj (#a:Type0) (#st:eqtype) = mgsub_inj #a #st #(trivial_preorder a) #(trivial_preorder a) (trivial_preorder a) (trivial_preorder a)
+
+[@unifier_hint_injective]
+inline_for_extraction
+type pointer (a:Type0) (st:eqtype) = b:buffer a st{length b == 1}
+
+inline_for_extraction
+type pointer_or_null (a:Type0) (st:eqtype) = b:buffer a st{if g_is_null b then True else length b == 1}
+
+inline_for_extraction let sub (#a:Type0) (#st:eqtype) = msub #a #st #(trivial_preorder a) #(trivial_preorder a) (trivial_preorder a)
+
+inline_for_extraction let offset (#a:Type0) (#st:eqtype) = moffset #a #st #(trivial_preorder a) #(trivial_preorder a) (trivial_preorder a)
+
+unfold let lbuffer (a:Type0) (#st:eqtype) (len:nat) = lmbuffer a st (trivial_preorder a) (trivial_preorder a) len
+
+inline_for_extraction let gcmalloc (#a:Type0) (#st:eqtype) = mgcmalloc #a #st #(trivial_preorder a)
+
+inline_for_extraction let malloc (#a:Type0) (#st:eqtype) = mmalloc #a #st #(trivial_preorder a)
+
+inline_for_extraction let alloca (#a:Type0) (#st:eqtype) = malloca #a #st #(trivial_preorder a)
+
+inline_for_extraction let alloca_of_list (#a:Type0) (#st:eqtype) = malloca_of_list #a #st #(trivial_preorder a)
+
+inline_for_extraction let gcmalloc_of_list (#a:Type0) (#st:eqtype) = mgcmalloc_of_list #a #st #(trivial_preorder a)
+
+module L = FStar.List.Tot
+
+unfold
+let assign_list_t #a #st (l: list a) = (b: buffer a st) -> HST.Stack unit
+  (requires (fun h0 ->
+    live h0 b /\
+    length b = L.length l))
+  (ensures (fun h0 _ h1 ->
+    live h1 b /\
+    (modifies (loc_buffer b) h0 h1) /\
+    as_seq h1 b == Seq.seq_of_list l))
+
+let rec assign_list #a (l: list a): assign_list_t l
+= fun b ->
+  match l with
+  | [] ->
+      let h = HST.get () in
+      assert (length b = 0);
+      assert (Seq.length (as_seq h b) = 0);
+      assert (Seq.equal (as_seq h b) (Seq.empty #a));
+      assert (Seq.seq_of_list [] `Seq.equal` Seq.empty #a)
+  | hd :: tl ->
+      let b_hd = sub b (index_zero b) (size_one b) in
+      let b_tl = offset b 1UL in
+      let h = HST.get () in
+      upd b_hd 0UL hd;
+      let h0 = HST.get () in
+      assign_list tl b_tl;
+      let h1 = HST.get () in
+      modifies_buffer_elim b_hd (loc_buffer b_tl) h0 h1;
+      assert (as_seq h1 b_hd == as_seq h0 b_hd);
+      assert (get h1 b_hd 0 == hd);
+      assert (as_seq h1 b_tl == Seq.seq_of_list tl);
+      assert (Seq.equal (as_seq h1 b) (Seq.append (as_seq h1 b_hd) (as_seq h1 b_tl)));
+      assert ((Seq.seq_of_list l) == (Seq.cons hd (Seq.seq_of_list tl)))
